Much more progress

LinearScan/Interval.hs
@@ -1,6 +1,3 @@
-{-# OPTIONS_GHC -cpp -fglasgow-exts #-}
-{- For Hugs, use the option -F"cpp -P -traditional" -}
-
 module LinearScan.Interval where
 
 
@@ -13,20 +10,7 @@ import qualified LinearScan.Utils
 import qualified LinearScan.Lib as Lib
 import qualified LinearScan.Logic as Logic
 import qualified LinearScan.Range as Range
-import qualified LinearScan.Eqtype as Eqtype
-import qualified LinearScan.Ssrnat as Ssrnat
 
-
-
---unsafeCoerce :: a -> b
-#ifdef __GLASGOW_HASKELL__
-import qualified GHC.Base as GHC.Base
-unsafeCoerce = GHC.Base.unsafeCoerce#
-#else
--- HUGS
-import qualified LinearScan.IOExts as IOExts
-unsafeCoerce = IOExts.unsafeCoerce
-#endif
 
 __ :: any
 __ = Prelude.error "Logical or arity value used"
@@ -76,19 +60,6 @@ intervalCoversPos d pos =
   (Prelude.&&) ((Prelude.<=) (intervalStart d) pos)
     ((Prelude.<=) ((Prelude.succ) pos) (intervalEnd d))
 
-intervalExtent :: IntervalDesc -> Prelude.Int
-intervalExtent d =
-  (Prelude.-) (intervalEnd d) (intervalStart d)
-
-coq_Interval_is_singleton :: IntervalDesc -> Prelude.Bool
-coq_Interval_is_singleton d =
-  (Prelude.&&)
-    (Eqtype.eq_op Ssrnat.nat_eqType (unsafeCoerce (Prelude.length (rds d)))
-      (unsafeCoerce ((Prelude.succ) 0)))
-    (Eqtype.eq_op Ssrnat.nat_eqType
-      (unsafeCoerce (Prelude.length (Range.ups ( (Prelude.head (rds d))))))
-      (unsafeCoerce ((Prelude.succ) 0)))
-
 intervalsIntersect :: IntervalDesc -> IntervalDesc -> Prelude.Bool
 intervalsIntersect i j =
   let {f = \x y -> Range.rangesIntersect ( x) ( y)} in
@@ -132,37 +103,31 @@ nextUseAfter d pos =
     (findIntervalUsePos d (\u ->
       (Prelude.<=) ((Prelude.succ) pos) (Range.uloc u)))
 
-firstUsePos :: IntervalDesc -> Prelude.Int
-firstUsePos d =
-  Range.uloc (Prelude.head (Range.ups ( (Prelude.head (rds d)))))
-
 firstUseReqReg :: IntervalDesc -> Prelude.Maybe Prelude.Int
 firstUseReqReg d =
   Lib.option_map ((Prelude..) Range.uloc Prelude.snd)
     (findIntervalUsePos d Range.regReq)
 
-lastUsePos :: IntervalDesc -> Prelude.Int
-lastUsePos d =
-  Range.uloc (Prelude.last (Range.ups ( (Prelude.last (rds d)))))
+data SplitPosition =
+   BeforePos Prelude.Int
+ | BeforeFirstUsePosReqReg
+ | EndOfLifetimeHole
 
-splitPosition :: IntervalDesc -> (Prelude.Maybe Prelude.Int) -> Prelude.Bool
-                 -> Prelude.Int
-splitPosition d before splitBeforeLifetimeHole =
-  let {initial = firstUsePos d} in
-  let {final = lastUsePos d} in
-  Prelude.max ((Prelude.succ) initial)
-    (Prelude.min final
-      (Lib.fromMaybe final (Lib.option_choose before (firstUseReqReg d))))
+splitPosition :: IntervalDesc -> SplitPosition -> Prelude.Maybe Prelude.Int
+splitPosition d pos =
+  case pos of {
+   BeforePos x -> Prelude.Just x;
+   BeforeFirstUsePosReqReg -> firstUseReqReg d;
+   EndOfLifetimeHole -> Prelude.Nothing}
 
 intervalSpan :: ([] Range.RangeDesc) -> Prelude.Int -> Prelude.Int ->
                 Prelude.Int -> Prelude.Int ->
                 ((,) (Prelude.Maybe IntervalDesc)
                 (Prelude.Maybe IntervalDesc))
 intervalSpan rs before iv ib ie =
-  let {f = \u -> (Prelude.<=) ((Prelude.succ) (Range.uloc u)) before} in
   (\ns nc l -> case l of [x] -> ns x; (x:xs) -> nc x xs)
     (\r ->
-    let {_top_assumption_ = Range.rangeSpan f ( r)} in
+    let {_top_assumption_ = Range.rangeSpan before ( r)} in
     let {
      _evar_0_ = \_top_assumption_0 ->
       let {
@@ -182,12 +147,16 @@ intervalSpan rs before iv ib ie =
            _evar_0_ __ __}
         in
         let {
-         _evar_0_0 = \_ ->
-          let {
-           _evar_0_0 = \_ -> (,) (Prelude.Just (Build_IntervalDesc iv ib ie
-            ((:[]) r))) Prelude.Nothing}
-          in
-           _evar_0_0 __}
+         _evar_0_0 = let {
+                      _evar_0_0 = let {
+                                   _evar_0_0 = \_ -> (,) (Prelude.Just
+                                    (Build_IntervalDesc iv (Range.rbeg ( r0))
+                                    (Range.rend ( r0)) ((:[]) ( r0))))
+                                    Prelude.Nothing}
+                                  in
+                                   _evar_0_0}
+                     in
+                      _evar_0_0}
         in
         case _top_assumption_1 of {
          Prelude.Just x -> (\_ -> _evar_0_ x);
@@ -198,14 +167,18 @@ intervalSpan rs before iv ib ie =
         let {
          _evar_0_0 = \r1 ->
           let {
-           _evar_0_0 = \_ -> (,) Prelude.Nothing (Prelude.Just
-            (Build_IntervalDesc iv ib ie ((:[]) r)))}
+           _evar_0_0 = let {
+                        _evar_0_0 = \_ -> (,) Prelude.Nothing (Prelude.Just
+                         (Build_IntervalDesc iv (Range.rbeg ( r1))
+                         (Range.rend ( r1)) ((:[]) ( r1))))}
+                       in
+                        _evar_0_0}
           in
-           _evar_0_0 __}
+           _evar_0_0}
         in
         let {_evar_0_1 = \_ -> Logic.coq_False_rec} in
         case _top_assumption_1 of {
-         Prelude.Just x -> (\_ -> _evar_0_0 x);
+         Prelude.Just x -> _evar_0_0 x;
          Prelude.Nothing -> _evar_0_1}}
       in
       case _top_assumption_0 of {
@@ -215,7 +188,7 @@ intervalSpan rs before iv ib ie =
     case _top_assumption_ of {
      (,) x x0 -> _evar_0_ x x0 __})
     (\r rs0 ->
-    let {_top_assumption_ = Range.rangeSpan f ( r)} in
+    let {_top_assumption_ = Range.rangeSpan before ( r)} in
     let {
      _evar_0_ = \_top_assumption_0 ->
       let {
@@ -224,15 +197,14 @@ intervalSpan rs before iv ib ie =
          _evar_0_ = \r1 ->
           let {
            _evar_0_ = \_ ->
-            let {
-             _evar_0_ = \_ _ ->
-              (Prelude.flip (Prelude.$)) __ (\_ -> (,) (Prelude.Just
-                (Build_IntervalDesc iv (Range.rbeg ( r0)) (Range.rend ( r0))
-                ((:[]) ( r0)))) (Prelude.Just (Build_IntervalDesc iv
-                (Range.rbeg ( r1)) (Range.rend ( (Prelude.last rs0))) ((:) r1
-                rs0))))}
-            in
-             _evar_0_ __ __}
+            (Prelude.flip (Prelude.$)) __ (\_ ->
+              let {
+               _evar_0_ = \_ -> (,) (Prelude.Just (Build_IntervalDesc iv
+                (Range.rbeg ( r0)) (Range.rend ( r0)) ((:[]) ( r0))))
+                (Prelude.Just (Build_IntervalDesc iv (Range.rbeg ( r1))
+                (Range.rend ( (Prelude.last rs0))) ((:) r1 rs0)))}
+              in
+               _evar_0_ __)}
           in
            _evar_0_ __}
         in
@@ -241,93 +213,130 @@ intervalSpan rs before iv ib ie =
           let {
            _evar_0_0 = \_ ->
             let {
-             _evar_0_0 = \_ ->
+             _top_assumption_2 = intervalSpan rs0 before iv
+                                   (Range.rbeg ( (Prelude.head rs0)))
+                                   (Range.rend ( (Prelude.last rs0)))}
+            in
+            let {
+             _evar_0_0 = \_top_assumption_3 ->
               let {
-               _top_assumption_2 = intervalSpan rs0 before iv
-                                     (Range.rbeg ( (Prelude.head rs0)))
-                                     (Range.rend ( (Prelude.last rs0)))}
-              in
-              let {
-               _evar_0_0 = \_top_assumption_3 ->
+               _evar_0_0 = \i1_1 _top_assumption_4 ->
                 let {
-                 _evar_0_0 = \i1_1 _top_assumption_4 ->
-                  let {
-                   _evar_0_0 = \i1_2 ->
-                    case i1_1 of {
-                     Build_IntervalDesc ivar0 ibeg0 iend0 rds0 ->
-                      let {
-                       _evar_0_0 = let {
-                                    _evar_0_0 = \_ _ ->
+                 _evar_0_0 = \i1_2 ->
+                  case i1_1 of {
+                   Build_IntervalDesc ivar0 ibeg0 iend0 rds0 ->
+                    let {
+                     _evar_0_0 = let {
+                                  _evar_0_0 = \_ ->
+                                   let {
+                                    _evar_0_0 = \_ ->
                                      let {
                                       _evar_0_0 = \_ ->
-                                       let {
-                                        _evar_0_0 = \_ ->
+                                       (Prelude.flip (Prelude.$)) __ (\_ ->
                                          let {
-                                          _evar_0_0 = (Prelude.flip (Prelude.$))
-                                                        __ (\_ ->
-                                                        let {
-                                                         _evar_0_0 = \_ _ ->
-                                                          (,) (Prelude.Just
-                                                          (Build_IntervalDesc
-                                                          ivar0
-                                                          (Range.rbeg ( r))
-                                                          iend0 ((:) r
-                                                          rds0)))
-                                                          (Prelude.Just
-                                                          i1_2)}
-                                                        in
-                                                         _evar_0_0 __)}
+                                          _evar_0_0 = let {
+                                                       _evar_0_0 = \_ _ _ ->
+                                                        (,) (Prelude.Just
+                                                        (Build_IntervalDesc
+                                                        ivar0
+                                                        (Range.rbeg ( r))
+                                                        iend0 ((:) r rds0)))
+                                                        (Prelude.Just i1_2)}
+                                                      in
+                                                       _evar_0_0 __}
                                          in
-                                          _evar_0_0}
-                                       in
-                                        _evar_0_0 __}
+                                          _evar_0_0)}
                                      in
                                       _evar_0_0 __}
                                    in
-                                    _evar_0_0}
-                      in
-                       _evar_0_0 __ __}}
-                  in
-                  let {
-                   _evar_0_1 = \_ ->
-                    let {
-                     _evar_0_1 = \_ _ _ -> (,) (Prelude.Just
-                      (Build_IntervalDesc iv (Range.rbeg ( r))
-                      (Range.rend ( (Prelude.last rs0))) ((:) r rs0)))
-                      Prelude.Nothing}
+                                    _evar_0_0 __}
+                                 in
+                                  _evar_0_0}
                     in
-                     _evar_0_1 __}
-                  in
-                  case _top_assumption_4 of {
-                   Prelude.Just x -> (\_ _ -> _evar_0_0 x);
-                   Prelude.Nothing -> _evar_0_1}}
+                     _evar_0_0 __}}
                 in
                 let {
-                 _evar_0_1 = \_top_assumption_4 ->
-                  let {
-                   _evar_0_1 = \i1_2 ->
+                 _evar_0_1 = \_ _ _ ->
+                  case i1_1 of {
+                   Build_IntervalDesc ivar0 ibeg0 iend0 rds0 ->
                     let {
-                     _evar_0_1 = \_ _ _ -> (,) (Prelude.Just
-                      (Build_IntervalDesc iv ib (Range.rend ( r)) ((:[]) r)))
-                      (Prelude.Just (Build_IntervalDesc iv
-                      (Range.rbeg ( (Prelude.head rs0)))
-                      (Range.rend ( (Prelude.last rs0))) rs0))}
+                     _evar_0_1 = let {
+                                  _evar_0_1 = \_ ->
+                                   (Prelude.flip (Prelude.$)) __ (\_ ->
+                                     (Prelude.flip (Prelude.$)) __ (\_ ->
+                                       let {
+                                        _evar_0_1 = \_ ->
+                                         let {
+                                          _evar_0_1 = \_ -> (,) (Prelude.Just
+                                           (Build_IntervalDesc ivar0
+                                           (Range.rbeg ( r)) iend0 ((:) r
+                                           rds0))) Prelude.Nothing}
+                                         in
+                                          _evar_0_1 __}
+                                       in
+                                        _evar_0_1 __))}
+                                 in
+                                  _evar_0_1}
                     in
-                     _evar_0_1 __}
-                  in
-                  let {_evar_0_2 = \_ _ _ -> Logic.coq_False_rec} in
-                  case _top_assumption_4 of {
-                   Prelude.Just x -> (\_ -> _evar_0_1 x);
-                   Prelude.Nothing -> _evar_0_2}}
+                     _evar_0_1 __}}
                 in
-                case _top_assumption_3 of {
-                 Prelude.Just x -> _evar_0_0 x;
+                case _top_assumption_4 of {
+                 Prelude.Just x -> (\_ -> _evar_0_0 x);
                  Prelude.Nothing -> _evar_0_1}}
               in
-              case _top_assumption_2 of {
-               (,) x x0 -> _evar_0_0 x x0 __ __ __}}
+              let {
+               _evar_0_1 = \_top_assumption_4 ->
+                let {
+                 _evar_0_1 = \i1_2 ->
+                  case i1_2 of {
+                   Build_IntervalDesc ivar0 ibeg0 iend0 rds0 ->
+                    let {
+                     _evar_0_1 = let {
+                                  _evar_0_1 = \_ ->
+                                   let {
+                                    _evar_0_1 = \_ _ ->
+                                     let {
+                                      _evar_0_1 = \_ ->
+                                       let {
+                                        _evar_0_1 = \_ ->
+                                         let {
+                                          _evar_0_1 = \_ ->
+                                           (Prelude.flip (Prelude.$)) __
+                                             (\_ -> (,) (Prelude.Just
+                                             (Build_IntervalDesc iv
+                                             (Range.rbeg ( r0))
+                                             (Range.rend ( r0)) ((:[])
+                                             ( r0)))) (Prelude.Just
+                                             (Build_IntervalDesc ivar0
+                                             (Range.rbeg
+                                               ( (Prelude.head rds0)))
+                                             (Range.rend
+                                               ( (Prelude.last rds0)))
+                                             rds0)))}
+                                         in
+                                          _evar_0_1 __}
+                                       in
+                                        _evar_0_1 __}
+                                     in
+                                      _evar_0_1 __}
+                                   in
+                                    _evar_0_1 __ __}
+                                 in
+                                  _evar_0_1}
+                    in
+                     _evar_0_1 __}}
+                in
+                let {_evar_0_2 = \_ _ _ -> Logic.coq_False_rec} in
+                case _top_assumption_4 of {
+                 Prelude.Just x -> (\_ _ _ -> _evar_0_1 x);
+                 Prelude.Nothing -> _evar_0_2}}
+              in
+              case _top_assumption_3 of {
+               Prelude.Just x -> _evar_0_0 x;
+               Prelude.Nothing -> _evar_0_1}}
             in
-             _evar_0_0 __}
+            case _top_assumption_2 of {
+             (,) x x0 -> _evar_0_0 x x0 __ __ __}}
           in
            _evar_0_0 __}
         in
@@ -340,8 +349,17 @@ intervalSpan rs before iv ib ie =
         let {
          _evar_0_0 = \r1 ->
           let {
-           _evar_0_0 = \_ -> (,) Prelude.Nothing (Prelude.Just
-            (Build_IntervalDesc iv ib ie ((:) r rs0)))}
+           _evar_0_0 = \_ ->
+            let {
+             _evar_0_0 = \_ ->
+              let {
+               _evar_0_0 = \_ -> (,) Prelude.Nothing (Prelude.Just
+                (Build_IntervalDesc iv (Range.rbeg ( r1))
+                (Range.rend ( (Prelude.last rs0))) ((:) r1 rs0)))}
+              in
+               _evar_0_0 __}
+            in
+             _evar_0_0 __}
           in
            _evar_0_0 __}
         in
@@ -357,44 +375,4 @@ intervalSpan rs before iv ib ie =
     case _top_assumption_ of {
      (,) x x0 -> _evar_0_ x x0 __})
     rs
-
-splitInterval :: Prelude.Int -> IntervalDesc ->
-                 ((,) IntervalDesc IntervalDesc)
-splitInterval before d =
-  let {
-   _evar_0_ = \iv ib ie rds0 ->
-    let {_top_assumption_ = intervalSpan rds0 before iv ib ie} in
-    let {
-     _evar_0_ = \_top_assumption_0 ->
-      let {
-       _evar_0_ = \i0 _top_assumption_1 ->
-        let {_evar_0_ = \i1 -> (,) i0 i1} in
-        let {
-         _evar_0_0 = \_ ->
-          let {_evar_0_0 = \_ -> Logic.coq_False_rec} in  _evar_0_0 __}
-        in
-        case _top_assumption_1 of {
-         Prelude.Just x -> (\_ -> _evar_0_ x);
-         Prelude.Nothing -> _evar_0_0}}
-      in
-      let {
-       _evar_0_0 = \_top_assumption_1 ->
-        let {
-         _evar_0_0 = \i1 ->
-          let {_evar_0_0 = \_ -> Logic.coq_False_rec} in  _evar_0_0 __}
-        in
-        let {_evar_0_1 = \_ -> Logic.coq_False_rec} in
-        case _top_assumption_1 of {
-         Prelude.Just x -> (\_ -> _evar_0_0 x);
-         Prelude.Nothing -> _evar_0_1}}
-      in
-      case _top_assumption_0 of {
-       Prelude.Just x -> _evar_0_ x;
-       Prelude.Nothing -> _evar_0_0}}
-    in
-    case _top_assumption_ of {
-     (,) x x0 -> _evar_0_ x x0 __}}
-  in
-  case d of {
-   Build_IntervalDesc x x0 x1 x2 -> _evar_0_ x x0 x1 x2}
 
