LinearScan/Lib.hs
@@ -7,23 +7,12 @@ import qualified Data.Ord
 import qualified Data.Functor.Identity
 import qualified LinearScan.Utils
 
-import qualified LinearScan.Logic as Logic
 import qualified LinearScan.Specif as Specif
 import qualified LinearScan.Eqtype as Eqtype
 
 
 __ :: any
 __ = Prelude.error "Logical or arity value used"
-
-ex_falso_quodlibet :: a1
-ex_falso_quodlibet =
-  Logic.coq_False_rect
-
-fromMaybe :: a1 -> (Prelude.Maybe a1) -> a1
-fromMaybe d mx =
-  case mx of {
-   Prelude.Just x -> x;
-   Prelude.Nothing -> d}
 
 option_map :: (a1 -> a2) -> (Prelude.Maybe a1) -> Prelude.Maybe a2
 option_map f x =
