LinearScan/Peano.hs
@@ -1,4 +1,8 @@
-module LinearScan.Peano where
+module LinearScan.LinearScan.LinearScan.LinearScan.LinearScan.Peano where
+
+
+
+
 
 
 import qualified Prelude
@@ -6,5 +10,25 @@ import qualified Data.List
 import qualified Data.Ord
 import qualified Data.Functor.Identity
 import qualified LinearScan.Utils
+
+import qualified LinearScan.Data.List as Data.List
+import qualified LinearScan.Data.Ord as Data.Ord
+import qualified LinearScan.Data.Functor.Identity as Data.Functor.Identity
+import qualified LinearScan.LinearScan.Utils as LinearScan.Utils
+
+import qualified LinearScan.LinearScan.Data.List as Data.List as LinearScan.Data.List as Data.List
+import qualified LinearScan.LinearScan.Data.Ord as Data.Ord as LinearScan.Data.Ord as Data.Ord
+import qualified LinearScan.LinearScan.Data.Functor.Identity as Data.Functor.Identity as LinearScan.Data.Functor.Identity as Data.Functor.Identity
+import qualified LinearScan.LinearScan.LinearScan.Utils as LinearScan.Utils as LinearScan.LinearScan.Utils as LinearScan.Utils
+
+import qualified LinearScan.LinearScan.LinearScan.Data.List as Data.List as LinearScan.Data.List as Data.List as LinearScan.LinearScan.Data.List as Data.List as LinearScan.Data.List as Data.List
+import qualified LinearScan.LinearScan.LinearScan.Data.Ord as Data.Ord as LinearScan.Data.Ord as Data.Ord as LinearScan.LinearScan.Data.Ord as Data.Ord as LinearScan.Data.Ord as Data.Ord
+import qualified LinearScan.LinearScan.LinearScan.Data.Functor.Identity as Data.Functor.Identity as LinearScan.Data.Functor.Identity as Data.Functor.Identity as LinearScan.LinearScan.Data.Functor.Identity as Data.Functor.Identity as LinearScan.Data.Functor.Identity as Data.Functor.Identity
+import qualified LinearScan.LinearScan.LinearScan.LinearScan.Utils as LinearScan.Utils as LinearScan.LinearScan.Utils as LinearScan.Utils as LinearScan.LinearScan.LinearScan.Utils as LinearScan.Utils as LinearScan.LinearScan.Utils as LinearScan.Utils
+
+import qualified LinearScan.LinearScan.LinearScan.LinearScan.Data.List as Data.List as LinearScan.Data.List as Data.List as LinearScan.LinearScan.Data.List as Data.List as LinearScan.Data.List as Data.List as LinearScan.LinearScan.LinearScan.Data.List as Data.List as LinearScan.Data.List as Data.List as LinearScan.LinearScan.Data.List as Data.List as LinearScan.Data.List as Data.List
+import qualified LinearScan.LinearScan.LinearScan.LinearScan.Data.Ord as Data.Ord as LinearScan.Data.Ord as Data.Ord as LinearScan.LinearScan.Data.Ord as Data.Ord as LinearScan.Data.Ord as Data.Ord as LinearScan.LinearScan.LinearScan.Data.Ord as Data.Ord as LinearScan.Data.Ord as Data.Ord as LinearScan.LinearScan.Data.Ord as Data.Ord as LinearScan.Data.Ord as Data.Ord
+import qualified LinearScan.LinearScan.LinearScan.LinearScan.Data.Functor.Identity as Data.Functor.Identity as LinearScan.Data.Functor.Identity as Data.Functor.Identity as LinearScan.LinearScan.Data.Functor.Identity as Data.Functor.Identity as LinearScan.Data.Functor.Identity as Data.Functor.Identity as LinearScan.LinearScan.LinearScan.Data.Functor.Identity as Data.Functor.Identity as LinearScan.Data.Functor.Identity as Data.Functor.Identity as LinearScan.LinearScan.Data.Functor.Identity as Data.Functor.Identity as LinearScan.Data.Functor.Identity as Data.Functor.Identity
+import qualified LinearScan.LinearScan.LinearScan.LinearScan.LinearScan.Utils as LinearScan.Utils as LinearScan.LinearScan.Utils as LinearScan.Utils as LinearScan.LinearScan.LinearScan.Utils as LinearScan.Utils as LinearScan.LinearScan.Utils as LinearScan.Utils as LinearScan.LinearScan.LinearScan.LinearScan.Utils as LinearScan.Utils as LinearScan.LinearScan.Utils as LinearScan.Utils as LinearScan.LinearScan.LinearScan.Utils as LinearScan.Utils as LinearScan.LinearScan.Utils as LinearScan.Utils
 
 
